---
title: "W203: Home Work 4 Suhas Gupta"
author: Suhas Gupta
Date: 10/1/2018
output:
  pdf_document: 
    latex_engine: xelatex
  html_document:
    df_print: paged
---

```{r setup, include=FALSE}
knitr::opts_chunk$set(echo = TRUE)
```

**Question 1:**

**(a)**  

The outcomes of a coin toss follows a binomial distribution with p.m.f given by:

$$
b(x;n,p) = \left\{
        \begin{array}{ll}
            {{n}\choose{k}} p^k(1-p)^k &, \quad x\in I \\
            0 &, \quad otherwise
        \end{array}
    \right.
$$
<center> where n: number of trials </center>
<center> p: probability of getting heads </center>

$$ \to p = 0.5 $$
$$ 1-p = 0.5 $$
Let h(X) denote the function that represents payout.

Expectation of earnings, 
$$  E(X) = \sum^3_0 {p(x)h(x)} $$
$$ = p(0)(0) + p(1)(2) + p(2)(4) + p(3)h(3) $$
$$ = (1/8)(0) + (3/8)(2) + (3/8)(4) + (1/8)h(3) $$
$$ But,\ E(X) = 6 (given) \\ $$  
Solving for h(3) gives, 

$$ \to h(3)  = 30 \\ $$
Expected earnings from getting 3 heads = **$30**

**(b)**

$$ F(X) = P(X \leq x) = \sum_{y:y\leq x}{P(y)}$$

$$ F(0) = P(y \leq 0) = \sum_{y:y\leq 0}{P(y)}) = \frac{1}{8} $$
$$ F(1) = P(y \leq 1) = \sum_{y:y\leq 1}{P(y)}) = \frac{1}{2} $$
$$ F(2) = P(y \leq 2) = \sum_{y:y\leq 2}{P(y)}) = \frac{7}{8} $$
$$ F(3) = P(y \leq 3) = \sum_{y:y\leq 3}{P(y)}) = 1 $$

Expression for cummulative probability F(Y): 

$$
F(Y) = \left\{
        \begin{array}{ll}
            0           &, \quad y < 0\\
            1/8 &, \quad 0 \leq y < 1\\
            1/2 &, \quad 1 \leq y < 2\\
            7/8 &, \quad 2 \leq y < 3\\
            1           &, \quad  3 < y\\
        \end{array}
    \right.
$$

**Question 2**  

p.d.f: 
$$
f(l) = \left\{
        \begin{array}{ll}
            0           &, \quad l \leq 0\\
            1/2         &, \quad 0 \leq l < 2\\
            0           &, \quad  2 < l\\
        \end{array}
    \right.
$$
**(a)**  

$$ F(l) = P(L \leq l) = \int_{-\infty}^{l} f(l) dl \\
 = \int_{0}^{l} {\frac{l}{2} dl}  = \frac{l^2}{4} 
$$
Thus c.d.f of L: 
$$ 
F(L) = \left\{
        \begin{array}{ll}
            0           &, \quad l \leq 0\\
            l^2/4 &, \quad 0 \leq l < 2\\
            1           &, \quad  2 < l\\
        \end{array}
    \right.
$$
**(b)**

$$ E(L) = \int_{-\infty}^{\infty} l \cdot f(l) dl $$
$$ = \int_{0}^{2} l \cdot \frac{l^2}{4} dl  $$
$$ = \frac{1}{12} l^3 \Big|_{0}^{2} $$

$$ = 0.67 $$ 

**Question 3**

**(a)**

c.r.v f(t),  
$$
f(t) = \left\{
        \begin{array}{ll}
            1           &, \quad 0 \leq x < 1\\
            0           &, \quad  otherwise\\
        \end{array}
    \right.
$$
c.d.f F(T), 
$$ F(T) = \int_{-\infty}^{t} f(t)dt = \int_{0}^{t} 1\ dt = t $$
Thus, 
$$
F(T) = \left\{
        \begin{array}{ll}
            0           &, \quad t < 0 \\
            t           &, \quad  0 \le t < 1\\
            1           &, \quad 1 \le t \\
        \end{array}
    \right.
$$
$$ g(t) = 100(1-t)^\frac{1}{2} $$
$$
E[g(T)] = \int_{-\infty}^{\infty} g(t) \cdot f(t) dt \\ 
= \int_{0}^{1} 100(1-t)\frac{1}{2} \cdot 1 dt
= 100 \frac{(1-t)^\frac{3}{2}}{\frac{3}{2}} \cdot (-1) \Big|_{0}^{1}\\
= \frac {200}{3} = 66.67
$$

**(b)**

***(i)***
$$ x = 100(1-t)^\frac{1}{2}\\
\to (1-t)^\frac{1}{2} = \frac {x}{100} \\
\to 1-t = \frac{x^2}{10^4}\\
\to t = 1-\frac{x^2}{10^4} ; 0 \le x \le 100
$$
***(ii)***
For $$ X \leq x, T \ge t $$
where 

$$ t = 1 - \frac{x^2}{10^4} $$

$$ 
P(T \ge t) = 1 - P(T \le t) = 1 - F(t) \\ 
 = 1-t\ ; \quad for\  0 \le 1
$$
***(iii)***

$$ F(X) = P(X \le x) = 1 - t = 1 - \Big(1-\frac{x^2}{10^4}\Big) = \frac{x^2}{10^4}$$
$$
F(X) = \left\{
        \begin{array}{ll}
            0           &, \quad x \leq 0 \\
           {x^2}/{10^4} &, \quad  0 \leq x < 100\\
            1           &, \quad 100 \leq x \\
        \end{array}
    \right.
$$
$$
F'(X) = \left\{
        \begin{array}{ll}
           {2x}/{10^4} &, \quad 0 \le x \le 100 \\
            0           &, otherwise \\
        \end{array}
    \right.
$$
$$ 
E(X) = \int_{0}^{100} {x \cdot \frac{2x}{10^4}dx} \\
 = \frac{2}{10^4} \cdot \frac{x^3}{3}\big|_{0}^{100} \\
 = \frac{200}{3} \\
 = 66.67
$$
 
 
**Question 4**
 
$$ X ; \quad t \in \mathbb{R} $$
$$ Y = (X -t)^2 $$

**(a)**

$$
E(Y) = \int_{-\infty}^{\infty}{(x-t)^2 f(x)dx} $$
$$ = E[(x-t)^2] $$
$$ = E[X^2+t^2-2Xt] $$
$$ = E(X^2)+E(t^2)-2E(Xt) $$
$$ = E(X^2)+t^2-2tE(X) $$
$$ to E(Y) = E(X^2)+t^2 - 2\mu_{X}t $$

**(b)**

$$
\frac{\partial E(Y)}{\partial t} $$
$$ = \frac{\partial E(X^2)}{\partial t} + 2t -2\mu_X = 2t-2\mu_X $$
$$ For\ minimum\ E(Y),\ 2t - 2\mu_X = 0 $$
$$ \to t = \mu_X  $$

**Question 5**

Given,
c.r.v X with p.d.f f(x)

& c.r.v Y = h(X) 

Let F(X) be the c.d.f of X,
i.e. f(x) = F'(X)

Also, 
$$ X = h^{-1}(X) $$
Let g(Y) be the p.d.f of Y 

Then, 

$$
F_Y(y) = P(Y \le y) \\
 = P(h(X) \le y) \\
 = \int_{h(x) < y}{f_X(x)dx} \\
$$
If h(X) is increasing, then 
$$
F_Y(y) = \int_{x \le h^{-1}(y)}{f_X(x)dx} \\
= \int_{-\infty}^{h^{-1}(y)} {f_X(x)dx} \\
= F_X\big(h^{-1}(y)\big)\\
$$
If h(X) is decreasing, thenm
$$
F_Y(y) = \int_{x \ge h^{-1}(y)}{f_X(x)dx} \\
= \int_{h^{-1}(y)}^{\infty} {f_X(x)dx} \\
= 1 - F_X\big(h^{-1}(y)\big) \\
$$
p.d.f of Y, 
$$ 
g(y) = \frac{d}{dy} F_Y(y)
$$

$$
\to g(y) =
    \left\{
        \begin{array}{ll}
            \frac{d}{dy} \Big(F_X(h^{-1}(y))\Big) &, \quad if\ h\ is\ increasing  \\
            \frac{d}{dy} \Big(1-F_X(h^{-1}(y))\Big) &, \quad\ if\ h\ is\ decreasing  \\
        \end{array}
    \right.
$$
Applying the chain rule of differentiation, we get 
$$
g(y) = 
\left\{
        \begin{array}{ll}
            f(h^{-1}(y))\Big(\frac{d}{dy}{h^{-1}(y)\Big)} &, \quad if\ h\ is\ increasing  \\
            f(h^{-1}(y))\Big(-\frac{d}{dy}{h^{-1}(y)\Big)} &, \quad if\ h\ is\ increasing  \\
        \end{array}
    \right.
$$
The above can be written in compact form as,

$$
g(y) = f(h^{-1}(y)) \cdot \Big|\frac{d}{dy}{h^{-1}(y)\Big|}
$$
